LynxTest/Modules/Erlang.lean
@@ -35,7 +35,6 @@ theorem reflexive_operators (a : Term) :
   simp [less_than_2, greater_than_2, less_than_or_equal_2, greater_than_or_equal_2,
     Term.true, Term.false]
 
-
 theorem tuple_equality :
     equal_2 (.tuple #[]) (.tuple #[]) = .ok Term.true ∧
     equal_2 (.tuple #[.integer 1]) (.tuple #[.integer 1, .nil]) = .ok Term.false ∧
